README.md
@@ -1,0 +1,19 @@
+# Formal Semantics of Ivy
+
+This repository contains some small-step structural operational semantics of the Ivy programming language. The semantics are given as formal inference rules and are implemented in Coq.
+
+## So Far
+- Syntax of most of the expressions and commands
+- Substitution functions
+- Typing of expressions and well-formedness of commands
+
+
+## TODOs
+- An `eval` function in Coq, and parsing so that I can test the Coq implementation. I might be able to leverage my use of `ocamlyacc` in the OCaml implementation to pass the same grammar to Coq.
+- Convert small steps for expressions and commands from OCaml to Coq
+- Prove type preservation/progress for expressions and commands
+- Prove that commands are well-formed if the underlying expressions are well-typed, and vice versa
+- The non-determinism operator might be weird in Coq because I used a random number generator in OCaml
+- Look over the data structures used again. I currently have a mess of different flavors of maps (some from `Maps.v` and some written by me). It would be very nice to swap some things out for things that act like sets. 
+- Incorporate assertions (axioms and pre-/post-conditions) into the interpreter
+- Quadruple check that what is down now works. A lot of the translation from OCaml to Coq was straightforward, but I got lazy and offloaded some to Copilot. The code looks fine, but I should double check that it works as intended.
